\documentclass[11pt]{article}
\usepackage{amsfonts,amssymb,amsmath,amsthm}
\usepackage{mathrsfs}
\usepackage{fullpage}

\newtheorem{theorem}{Theorem}%[section]
\newtheorem{lemma}[theorem]{Lemma}
\newtheorem{proposition}[theorem]{Proposition}
\newtheorem{remark}[theorem]{Remark}
\newtheorem{procedure}[theorem]{Procedure}
\newtheorem{definition}[theorem]{Definition}
\newtheorem{conjecture}[theorem]{Conjecture}
\newtheorem{observation}[theorem]{Observation}
\newtheorem{construction}[theorem]{Construction}
\newtheorem{claim}[theorem]{Claim}
\newtheorem{fact}[theorem]{Fact}
\newtheorem{notation}[theorem]{Notation}

\newtheorem{statement}{Statement}%[section]
\newtheorem{problem}[statement]{Problem}
\newtheorem{question}[statement]{Question}

\newtheorem{case}{Case}
\newtheorem{example}{Example}
\newtheorem{note}{Note}

\newcommand{\pow}[1]{\mathscr{P}(#1)}

\renewcommand{\labelenumi}{\emph{(\roman{enumi})}}
\setcounter{statement}{-1}


\begin{document}

\author{Robert Ritchie}
\title{MTH 331 -- Lemma 41}
\date{\today}

\maketitle
Let U and V be finite dimensional vector spaces (over the same field F) and let $T : U \rightarrow V$ be a linear transformation. If $B = \{u_{1}, . . . , u_{k}\}$ is a basis for U, then for all $u \in U$, there exists unique $a_{1}, . . . , a_{k} \in F$ such that $T(u) = a_{1}T(u_{1}) + ... + a_{k}T(u_{k})$.

\begin{proof} 
Suppose $B = \{u_{1}, . . . , u_{k}\}$ is a basis for U.
Let $x \in U$ then there exist scalars $\alpha_{1},...,\alpha_{k},\beta_{1},...,\beta_{k} \in F$ such that $x=\alpha_{1}u_{1}+...+\alpha_{k}u_{k}=\beta_{1}u_{1}+...+\beta_{k}u_{k}$.
$\rightarrow (\alpha_{1}-\beta_{1})u_{1}+...+(\alpha_{k}-\beta_{k})u_{k}=0$ Since the basis is independant, the only linear combination of its vectors that makes zero is the one where all of the scalars are zero so $\alpha_{1}-\beta_{1}=...=\alpha_{k}-\beta_{k}=0 \rightarrow \alpha_{1}=\beta_{1},...,\alpha_{k}=\beta_{k}$ \\ 
Since  $B = \{u_{1}, . . . , u_{k}\}$ is a basis for U, $\forall u \in U, \exists !\alpha_{1},...,\alpha_{k}\in F$ such that $u=\alpha_{1}u_{1}+...+\alpha_{k}u_{k}$.
\begin{align*}
T(u)&=T(\alpha_{1}u_{1}+...+\alpha_{k}u_{k}) \\
&=\alpha_{1}T(u_{1})+..+\alpha_{k}T(u_{k})
\end{align*}

\end{proof}

\end{document} 