\documentclass[11pt]{article}
\usepackage{amsfonts,amssymb,amsmath,amsthm}
\usepackage{mathrsfs}
\usepackage{fullpage}

\newtheorem{theorem}{Theorem}%[section]
\newtheorem{lemma}[theorem]{Lemma}
\newtheorem{proposition}[theorem]{Proposition}
\newtheorem{remark}[theorem]{Remark}
\newtheorem{procedure}[theorem]{Procedure}
\newtheorem{definition}[theorem]{Definition}
\newtheorem{conjecture}[theorem]{Conjecture}
\newtheorem{observation}[theorem]{Observation}
\newtheorem{construction}[theorem]{Construction}
\newtheorem{claim}[theorem]{Claim}
\newtheorem{fact}[theorem]{Fact}
\newtheorem{notation}[theorem]{Notation}

\newtheorem{statement}{Statement}%[section]
\newtheorem{problem}[statement]{Problem}
\newtheorem{question}[statement]{Question}

\newtheorem{case}{Case}
\newtheorem{example}{Example}
\newtheorem{note}{Note}

\newcommand{\pow}[1]{\mathscr{P}(#1)}

\renewcommand{\labelenumi}{\emph{(\roman{enumi})}}
\setcounter{statement}{-1}


\begin{document}

\author{Robert Ritchie}
\title{MTH 331 -- Theorem 39}
\date{\today}

\maketitle

Let T be a linear transformation on a finite vector space V. Then $dim(V)=dim(kerT)+dim(ranT)$.
\begin{proof} 
Let $B'=\{k_1,...,k_m\}$ be a basis for kerT. Since $B'$ is independant, we can extend it to a basis for V say $B=\{k_1,...,k_m,u_1,...,u_n\}$. 
Let $U=\{Tu_1,...,Tu_n\}$
 Let $w \in ranT$, this implies that $\exists v \in V$ such that $Tv=w \rightarrow \exists \alpha_1,...,\alpha_m,\beta_1,...,\beta_n \in F$ such that
\begin{align*} 
v&=\alpha_1k_1+...+\alpha_mk_m+\beta_1u_1+...+\beta_nu_n\\
Tv&=T(\alpha_1k_1+...+\alpha_mk_m+\beta_1u_1+...+\beta_nu_n) \\
w&=\alpha_1Tk_1+...+\alpha_mTk_m+\beta_1Tu_1+...+\beta_nTu_n \\
&=\beta_1Tu_1+...+\beta_nTu_n \\
 &\rightarrow \bigvee \{Tu_1,...,Tu_n\}=ranT
\end{align*}
Let $\gamma_1,...,\gamma_n \in F$. Suppose
$T\gamma_1u_1+...+T\gamma_nu_n=0$ \\
$ \rightarrow T(\gamma_1u_1+...+\gamma_nu_n)=0 \\
\rightarrow \gamma_1u_1+...+\gamma_nu_n \in kerT \\
 \rightarrow \gamma_1u_1+...+\gamma_nu_n=\beta_1k_1+...+\beta_mk_m$ and since $\{k_1,...,k_m,u_1,...,u_n\}$ is independant, $\gamma_1=...=\gamma_n=\beta_1=...=\beta_n=0$ so $\{Tu_1,...,Tu_n\}$ is independant.
\end{proof}

\end{document} 